设 $\vec{A}=A_{x}\hat{i}+A_{y}\hat{j}+A_{z}\hat{k}$ 是调和场，有
$$
\nabla \cdot \vec{A}=\frac{\partial A_{x}}{\partial x}+\frac{\partial A_{y}}{\partial y}+\frac{\partial A_{z}}{\partial z}=0
$$
$$
\nabla \times \vec{A}=\begin{vmatrix}
\hat{i}&\hat{j}&\hat{k} \\
\dfrac{{\partial}}{{\partial x}}&\dfrac{{\partial}}{{\partial y}}&\dfrac{{\partial}}{{\partial z}}\\
A_{x}&A_{y}&A_{z}
\end{vmatrix}=0
$$
得 $\dfrac{{\partial A_{z}}}{{\partial y}}=\dfrac{{\partial A_{y}}}{{\partial z}}\text{{，}}\dfrac{{\partial A_{z}}}{{\partial y}}=\dfrac{{\partial A_{y}}}{{\partial z}}\text{{，}}\dfrac{{\partial A_{z}}}{{\partial y}}=\dfrac{{\partial A_{y}}}{{\partial z}}$
以 $A_{x}$ 为例，有
$$
\begin{aligned}
\nabla^{2}A_{x}&=\frac{{\partial^{2}A_{x}}}{{\partial x^{2}}}+\frac{{\partial^{2}A_{y}}}{{\partial y^{2}}}+\frac{{\partial^{2}A_{z}}}{{\partial z^{2}}}\\
&=\frac{{\partial}}{{\partial x}}\left(-\frac{{\partial A_{y}}}{{\partial y}}-\frac{{\partial A_{z}}}{{\partial z}}\right)+\frac{{\partial}}{{\partial y}}\left(\frac{{\partial A_{x}}}{{\partial y}}\right)+\frac{{\partial}}{{\partial z}}\left(\frac{{\partial A_{x}}}{{\partial z}}\right)\\
&=\frac{{\partial}}{{\partial y}}\left( \frac{{\partial A_{x}}}{{\partial y}}-\frac{{\partial A_{y}}}{{\partial x}} \right)+\frac{{\partial}}{{\partial z}}\left( \frac{{\partial A_{x}}}{{\partial z}}-\frac{{\partial A_{z}}}{{\partial x}} \right)\\
&=0
\end{aligned}
$$
$$
\begin{align}
\nabla^{2}A_{x}&=\frac{{\partial^{2}A_{x}}}{{\partial x^{2}}}+\frac{{\partial^{2}A_{y}}}{{\partial y^{2}}}+\frac{{\partial^{2}A_{z}}}{{\partial z^{2}}}\\
&=\frac{{\partial}}{{\partial x}}\left(-\frac{{\partial A_{y}}}{{\partial y}}-\frac{{\partial A_{z}}}{{\partial z}}\right)+\frac{{\partial}}{{\partial y}}\left(\frac{{\partial A_{x}}}{{\partial y}}\right)+\frac{{\partial}}{{\partial z}}\left(\frac{{\partial A_{x}}}{{\partial z}}\right)\\
&=\frac{{\partial}}{{\partial y}}\left( \frac{{\partial A_{x}}}{{\partial y}}-\frac{{\partial A_{y}}}{{\partial x}} \right)+\frac{{\partial}}{{\partial z}}\left( \frac{{\partial A_{x}}}{{\partial z}}-\frac{{\partial A_{z}}}{{\partial x}} \right)\\
&=0
\end{align}
$$
设\(\vec{A} = A_x\hat{i} + A_y\hat{j} + A_z\hat{k}\)是调和场，有
\[
\nabla \cdot \vec{A} = \frac{\partial A_x}{\partial x} + \frac{\partial A_y}{\partial y} + \frac{\partial A_z}{\partial z} = 0
\]
\[
\nabla \times \vec{A} = \begin{vmatrix}
\hat{i} & \hat{j} & \hat{k} \\
\frac{\partial}{\partial x} & \frac{\partial}{\partial y} & \frac{\partial}{\partial z} \\
A_x & A_y & A_z
\end{vmatrix} = 0
\]
得\(\frac{\partial A_z}{\partial y} = \frac{\partial A_y}{\partial z}\)，\(\frac{\partial A_z}{\partial y} = \frac{\partial A_y}{\partial z}\)，\(\frac{\partial A_z}{\partial y} = \frac{\partial A_y}{\partial z}\)
以\(A_x\)为例，有
\[
\begin{align*}
\nabla^2 A_x &= \frac{\partial^2 A_x}{\partial x^2} + \frac{\partial^2 A_y}{\partial y^2} + \frac{\partial^2 A_z}{\partial z^2} \\
&= \frac{\partial}{\partial x}\left(-\frac{\partial A_y}{\partial y} - \frac{\partial A_z}{\partial z}\right) + \frac{\partial}{\partial y}\left(\frac{\partial A_x}{\partial y}\right) + \frac{\partial}{\partial z}\left(\frac{\partial A_x}{\partial z}\right) \\
&= \frac{\partial}{\partial y}\left(\frac{\partial A_x}{\partial y} - \frac{\partial A_y}{\partial x}\right) + \frac{\partial}{\partial z}\left(\frac{\partial A_x}{\partial z} - \frac{\partial A_z}{\partial x}\right) \\
&= 0
\end{align*}
\]
\[
\begin{align*}
\nabla^2 A_x &= \frac{\partial^2 A_x}{\partial x^2} + \frac{\partial^2 A_y}{\partial y^2} + \frac{\partial^2 A_z}{\partial z^2} \quad (1) \\
&= \frac{\partial}{\partial x}\left(-\frac{\partial A_y}{\partial y} - \frac{\partial A_z}{\partial z}\right) + \frac{\partial}{\partial y}\left(\frac{\partial A_x}{\partial y}\right) + \frac{\partial}{\partial z}\left(\frac{\partial A_x}{\partial z}\right) \quad (2) \\
&= \frac{\partial}{\partial y}\left(\frac{\partial A_x}{\partial y} - \frac{\partial A_y}{\partial x}\right) + \frac{\partial}{\partial z}\left(\frac{\partial A_x}{\partial z} - \frac{\partial A_z}{\partial x}\right) \quad (3) \\
&= 0 \quad (4)
\end{align*}
\]